Require sequential consistency in specs:

Core/Specs.v
@@ -1,5 +1,11 @@
 From LHL.Core Require Import
-    Program.
+  Program.
+
+From Coq Require Import
+  Arith.PeanoNat.
+
+From LHL.Util Require Import
+  TransUtil.
 
 Definition ThreadName := nat.
 
@@ -10,26 +16,44 @@ Arguments Event : clear implicits.
 
 Definition ThreadEvent (E : ESig) : Type := ThreadName * Event E.
 
-Record Spec {E : ESig} : Type :=  {
-    State : Type;
-    Step : State -> ThreadEvent E -> State -> Prop;
-    Init : State
+Definition ActiveMap (E : ESig) := ThreadName -> option {A & E A}.
+
+Inductive SeqConsistent {E} : ActiveMap E -> list (ThreadEvent E) -> Prop :=
+| SCNil a : SeqConsistent a nil
+| SCCall (a a' : ActiveMap E) i A (m : E A) p :
+    a i = None ->
+    a' i = Some (existT _ _ m) ->
+    SeqConsistent a' p ->
+    SeqConsistent a ((i, CallEv m) :: p)
+| SCRet (a a' : ActiveMap E) i A (m : E A) v p :
+    a i = Some (existT _ _ m) ->
+    a' i = None ->
+    SeqConsistent a' p ->
+    SeqConsistent a ((i, RetEv m v) :: p).
+
+Record Spec {E} : Type := {
+  State : Type;
+  Step : State -> ThreadEvent E -> State -> Prop;
+  Init : State;
+  seq_cons : forall p s,
+    Steps Step Init p s ->
+    SeqConsistent (fun _ => None) p
 }.
 Arguments Spec : clear implicits.
 
 Record Layer {E F : ESig} : Type := mkLayer {
-    USpec : Spec E;
-    LImpl : Impl E F; 
+  USpec : Spec E;
+  LImpl : Impl E F; 
 }.
 Arguments Layer : clear implicits.
 Arguments mkLayer {E F} USpec LImpl.
 Notation "x :> y" := (mkLayer x y) (at level 80, right associativity).
 
 Definition idLayer {E : ESig} (spec : Spec E) :=
-    {|
-        USpec := spec;
-        LImpl := idImpl
-    |}.
+  {|
+    USpec := spec;
+    LImpl := idImpl
+  |}.
 
 (* Layer Events *)
 
@@ -46,8 +70,8 @@ Definition ThreadLEvent E F : Type := nat * LEvent E F.
 (* Layer Composition *)
 
 Definition layVComp {E F G} (lay : Layer E F) (impl : Impl F G) : Layer E G :=
-    {|
-        USpec := lay.(USpec);
-        LImpl := implVComp lay.(LImpl) impl
-    |}.
+  {|
+    USpec := lay.(USpec);
+    LImpl := implVComp lay.(LImpl) impl
+  |}.
 Notation "x :|> y" := (layVComp x y) (at level 80, right associativity).
