Core/Tensor.v
@@ -2,32 +2,91 @@ From LHL.Core Require Import
   Program
   Specs.
 
+From LHL.Util Require Import
+  Util
+  TransUtil
+  Tactics.
+
+From Coq Require Import
+  Program.Equality.
+
+Definition TensorActive EL ER := ThreadName -> option ({A & (EL |+| ER) A}).
+
+Record TensorState {EL ER} {specL : Spec EL} {specR : Spec ER} := MkTS {
+  TActive : TensorActive EL ER;
+  LState : specL.(State);
+  RState : specR.(State)
+}.
+Arguments TensorState {EL ER} specL specR.
+
 Section Tensor.
-  Context {EL ER}
-          (specL : Spec EL)
-          (specR : Spec ER).
 
-  Definition StepTensor st (ev : ThreadEvent (EL |+| ER)) st' :=
-    match ev with
-      | (i, CallEv m) => 
-          match m with
-          |  inl m' => specL.(Step) (fst st) (i, CallEv m') (fst st') /\ (snd st = snd st')
-          |  inr m' => specR.(Step) (snd st) (i, CallEv m') (snd st') /\ (fst st = fst st')
-          end
-      | (i, RetEv m n) => 
-          match m with
-          | inl m' => specL.(Step) (fst st) (i, RetEv m' n) (fst st') /\ (snd st = snd st')
-          | inr m' => specR.(Step) (snd st) (i, RetEv m' n) (snd st') /\ (fst st = fst st')
-          end
-    end.
+Context {EL ER}
+        (specL : Spec EL)
+        (specR : Spec ER).
 
-  Definition tensorSpec : Spec (EL |+| ER) :=
-    {|
-      State := specL.(State) * specR.(State);
-      Step := StepTensor;
-      Init := (specL.(Init), specR.(Init))
-    |}.
+Definition TensorStep st (ev : ThreadEvent (EL |+| ER)) st' :=
+  match ev with
+    | (i, CallEv m) => 
+        match m with
+        |  inl m' =>
+          specL.(Step) st.(LState) (i, CallEv m') st'.(LState) /\
+          st.(TActive) i = None /\ st'.(TActive) i = Some (existT _ _ m) /\
+          differ_pointwise st.(TActive) st'.(TActive) i /\
+          st.(RState) = st'.(RState)
+        |  inr m' =>
+          specR.(Step) st.(RState) (i, CallEv m') st'.(RState) /\
+          st.(TActive) i = None /\ st'.(TActive) i = Some (existT _ _ m) /\
+          differ_pointwise st.(TActive) st'.(TActive) i /\
+          st.(LState) = st'.(LState)
+        end
+    | (i, RetEv m n) => 
+        match m with
+        | inl m' =>
+          specL.(Step) st.(LState) (i, RetEv m' n) st'.(LState) /\
+          st.(TActive) i = Some (existT _ _ m) /\ st'.(TActive) i = None /\
+          differ_pointwise st.(TActive) st'.(TActive) i /\
+          st.(RState) = st'.(RState)
+        | inr m' =>
+          specR.(Step) st.(RState) (i, RetEv m' n) st'.(RState) /\
+          st.(TActive) i = Some (existT _ _ m) /\ st'.(TActive) i = None /\
+          differ_pointwise st.(TActive) st'.(TActive) i /\
+          st.(LState) = st'.(LState)
+        end
+  end.
+
+Program Definition tensorSpec : Spec (EL |+| ER) :=
+  {|
+    State := TensorState specL specR;
+    Step := TensorStep;
+    Init := {|
+      TActive _ := None;
+      LState := Init specL;
+      RState := Init specR
+    |}
+  |}.
+
+Next Obligation.
+generalize dependent (fun _ : ThreadName => @None {A : Type & (EL |+| ER) A}).
+generalize dependent (Init specL). generalize dependent (Init specR).
+induction p; cbn; intros.
+{
+  constructor.
+}
+{
+  dependent destruction H. destruct st''.
+  destruct a, e, m; cbn in *; destruct_all;
+  eapply IHp in H0; clear IHp.
+  econstructor. easy. exact H2. easy.
+  econstructor. easy. exact H2. easy.
+  econstructor. easy. exact H2. easy.
+  econstructor. easy. exact H2. easy.
+}
+Qed.
+
 End Tensor.
+
+Arguments MkTS {EL ER specL specR}.
 
 Definition tensorImpl 
   {EL FL} (ML : Impl EL FL) {ER FR} (MR : Impl ER FR) : Impl (EL |+| ER) (FL |+| FR) :=
